implement new tuples handling
and update non-tuples Gencot theories

isa/Gencot_CArray.thy
@@ -3,60 +3,95 @@ theory Gencot_CArray
     Gencot_Default
 begin
 
-text \<open>Define the array functions for fixed lists\<close>
-
-definition getArr' :: "('n::len, 'el) FixedList \<Rightarrow> 'idx::len word \<Rightarrow> 'el"
-  where 
-    "getArr' lst idx \<equiv>
-      if unat idx >= LENGTH('n) then hd (Rep_FixedList lst)
-      else (nth (Rep_FixedList lst) (unat idx))"
-
-definition setArr' :: "('n::len, 'el) FixedList \<Rightarrow> 'idx::len word \<Rightarrow> 'el \<Rightarrow> ('n, 'el) FixedList"
-  where
-    "setArr' lst idx elm \<equiv> 
-      if unat idx >= LENGTH('n) then lst
-      else (Abs_FixedList (list_update (Rep_FixedList lst) (unat idx) elm))"
-
-definition modifyArr' :: "('n::len, 'el) FixedList \<Rightarrow> 'idx::len word \<Rightarrow> (('el, 'arg) RR \<Rightarrow> ('el, 'arg) RR) \<Rightarrow> 'arg \<Rightarrow> (('n, 'el) FixedList, 'arg) RR"
-  where
-    "modifyArr' lst idx chf inp \<equiv> 
-      if unat idx >= LENGTH('n) then RR.make lst inp
-      else let l = Rep_FixedList lst; elm = nth l (unat idx); chres = chf(RR.make elm inp)
-        in RR.make (Abs_FixedList (list_update l (unat idx) (RR.p1\<^sub>f chres))) (RR.p2\<^sub>f chres)"
-
-definition modifyArrDflt' :: "('n::len, 'el) FixedList \<Rightarrow> 'idx::len word \<Rightarrow>(('el, 'arg) RR \<Rightarrow> ('el, 'out) RR) \<Rightarrow> 'arg \<Rightarrow> (('n, 'el) FixedList, 'out) RR"
-  where
-    "modifyArrDflt' lst idx chf inp \<equiv> 
-      if unat idx >= LENGTH('n) then RR.make lst (defaultVal ())
-      else let l = Rep_FixedList lst; elm = nth l (unat idx); chres = chf(RR.make elm inp)
-        in RR.make (Abs_FixedList (list_update l (unat idx) (RR.p1\<^sub>f chres))) (RR.p2\<^sub>f chres)"
+section \<open>Gencot Array Operations\<close>
 
 text \<open>
-  This locale has the wrapper record access and constructor as parameters.
-  It defines the array functions for the wrapper record and proves some useful lemmas.\<close>
+Non-tuples form. For detailed description see theory \<open>Gencot_CArray_Tuples\<close>.
+\<close>
 
-locale CArrFuns = 
-  fixes 
-    fld :: "'arr \<Rightarrow> ('n::len, 'el) FixedList" and 
-    wrp :: "('n, 'el) FixedList \<Rightarrow> 'arr" 
+subsection \<open>Definitions for the Gencot Array Operations\<close>
+
+consts
+  toPtr :: "'el \<Rightarrow> 'pel"
+  frPtr :: "'pel \<Rightarrow> 'el"
+
+locale CArrayDefs = 
+  fixes arr :: "'carr \<Rightarrow> 'el list"
+    and arr_update :: "('el list \<Rightarrow> 'el list) \<Rightarrow> 'carr \<Rightarrow> 'carr"
+    and siz :: "'carr \<Rightarrow> nat"
+    and idxtypespec :: "('m::len) word"
 begin
-definition getArrFxd :: "('arr, 32 word) RR \<Rightarrow> 'el"
-  where "getArrFxd arg \<equiv>
-  let arr = RR.p1\<^sub>f arg; idx = RR.p2\<^sub>f arg 
-  in getArr' (fld arr) idx"
-definition setArrFxd :: "('arr, (32 word, 'el) RR) RR \<Rightarrow> ('arr, unit) RR"
-  where "setArrFxd arg \<equiv>
-  let arr = RR.p1\<^sub>f arg; idx = RR.p1\<^sub>f (RR.p2\<^sub>f arg); elm = RR.p2\<^sub>f (RR.p2\<^sub>f arg) 
-  in RR.make (wrp(setArr' (fld arr) idx elm)) ()"
-definition modifyArrFxd :: "('arr, (32 word, ('el, 'arg) RR \<Rightarrow> ('el, 'arg) RR, 'arg) Tup3) RR \<Rightarrow> ('arr, 'arg) RR"
-  where "modifyArrFxd arg \<equiv>
-  let arr = RR.p1\<^sub>f arg; idx = Tup3.p1\<^sub>f (RR.p2\<^sub>f arg); chf = Tup3.p2\<^sub>f (RR.p2\<^sub>f arg); inp = Tup3.p3\<^sub>f (RR.p2\<^sub>f arg); fres = modifyArr' (fld arr) idx chf inp 
-  in RR.make (wrp (RR.p1\<^sub>f fres)) (RR.p2\<^sub>f fres)"
-definition modifyArrDfltFxd :: "('arr, (32 word, ('el, 'arg) RR \<Rightarrow> ('el, 'out) RR, 'arg) Tup3) RR \<Rightarrow> ('arr, 'out) RR"
-  where "modifyArrDfltFxd arg \<equiv>
-  let arr = RR.p1\<^sub>f arg; idx = Tup3.p1\<^sub>f (RR.p2\<^sub>f arg); chf = Tup3.p2\<^sub>f (RR.p2\<^sub>f arg); inp = Tup3.p3\<^sub>f (RR.p2\<^sub>f arg); fres = modifyArrDflt' (fld arr) idx chf inp
-  in RR.make (wrp (RR.p1\<^sub>f fres)) (RR.p2\<^sub>f fres)"
+definition getArr :: "('carr, 'm word) Tup2 \<Rightarrow> 'el"
+  where "getArr arg \<equiv> let c = p1Tup2 arg; i = p2Tup2 arg in 
+            if unat i \<ge> siz c then hd (arr c) else (nth (arr c) (unat i))"
+definition setArr :: "('carr, 'm word, 'el) Tup3 \<Rightarrow> ('carr, unit) Tup2"
+  where "setArr arg \<equiv> let c = p1Tup3 arg; i = p2Tup3 arg; e = p3Tup3 arg in 
+            makeTup2 (if unat i \<ge> siz c then c else arr_update (\<lambda>a. (list_update a (unat i) e)) c) ()"
+definition modifyArr :: "('carr, 'm word, (('el, 'arg) Tup2 \<Rightarrow> ('el, 'out) Tup2), 'arg) Tup4 \<Rightarrow> ('carr, 'out) Tup2"
+  where "modifyArr arg \<equiv> 
+    let c = p1Tup4 arg; idx = p2Tup4 arg; u = p3Tup4 arg; inp = p4Tup4 arg;
+        i = (if unat idx \<ge> siz c then 0 else unat idx);
+        ures = u (makeTup2 (nth (arr c) i) inp) 
+    in makeTup2 (arr_update (\<lambda>a. (list_update a i (p1Tup2 ures))) c) (p2Tup2 ures)"
+definition modrefArr :: "('carr, 'm word, (('pel, 'arg) Tup2 \<Rightarrow> ('pel, 'out) Tup2 ), 'arg) Tup4 \<Rightarrow> ('carr, 'out) Tup2"
+  where "modrefArr arg \<equiv> 
+    let c = p1Tup4 arg; idx = p2Tup4 arg; u = p3Tup4 arg; inp = p4Tup4 arg; 
+        i = (if unat idx \<ge> siz c then 0 else unat idx); 
+        ures = u(makeTup2 (toPtr (nth (arr c) i)) inp)
+    in makeTup2 (arr_update (\<lambda>a. (list_update a i (frPtr (p1Tup2 ures)))) c) (p2Tup2 ures)"
+end
 
+subsubsection \<open>Explicitly sized arrays\<close>
+
+locale ESArrBase
+begin
+definition arr :: "'el CArrES\<^sub>T \<Rightarrow> 'el list" 
+  where "arr \<equiv> p1Tup2"
+definition arr_update :: "('el list \<Rightarrow> 'el list) \<Rightarrow> 'el CArrES\<^sub>T \<Rightarrow> 'el CArrES\<^sub>T"
+  where "arr_update \<equiv> p1Tup2_update"
+definition siz :: "'el CArrES\<^sub>T \<Rightarrow> nat" 
+  where "siz \<equiv> (unat \<circ> p2Tup2)"
+definition carr :: "'el list \<Rightarrow> 'el CArrES\<^sub>T" 
+  where "carr \<equiv> \<lambda>a. makeTup2 a (of_nat (length a))"
+end
+
+locale ESArrDefs = ESArrBase
+begin
+sublocale CArrayDefs arr arr_update siz "0::64 word" .
+end
+
+subsubsection \<open>Fixed sized arrays\<close>
+
+locale FxdArrBase = 
+  fixes arr :: "'carr \<Rightarrow> 'el list"
+    and carr :: "'el list \<Rightarrow> 'carr"
+    and fxdsiz :: "nat"
+begin
+
+definition siz :: "'carr \<Rightarrow> nat"
+  where fxdsiz_def: "siz c \<equiv> fxdsiz"
+definition arr_update :: "('el list \<Rightarrow> 'el list) \<Rightarrow> 'carr \<Rightarrow> 'carr"
+  where "arr_update u \<equiv> carr \<circ> u \<circ> arr"
+
+definition toCAES :: "'carr \<Rightarrow> 'el CArrES\<^sub>T"
+  where "toCAES a \<equiv> makeTup2 (arr a) (of_nat (fxdsiz))"
+definition fromCAES :: "'el CArrES\<^sub>T \<Rightarrow> 'carr"
+  where "fromCAES aes \<equiv> carr (p1Tup2 aes)"
+definition rotoCAES :: "'carr \<Rightarrow> 'el CArrES\<^sub>T"
+  where [simp]: "rotoCAES a \<equiv> toCAES a"
+definition rofromCAES :: "'el CArrES\<^sub>T \<Rightarrow> 'carr"
+  where [simp]: "rofromCAES aes \<equiv> fromCAES aes"
+
+end
+
+locale FxdArrDefs = FxdArrBase arr carr fxdsiz
+  for arr :: "'carr \<Rightarrow> 'el list"
+  and carr :: "'el list \<Rightarrow> 'carr"
+  and fxdsiz :: "nat"
++ 
+fixes idxtypespec :: "('m::len) word"
+begin
+sublocale CArrayDefs arr arr_update siz idxtypespec .
 end
 
 end
