isa/CogentCommon_common.thy
@@ -2,24 +2,69 @@ theory CogentCommon_common
   imports ShallowShared
 begin
 
+section \<open>Iteration Functions\<close>
+
+text \<open>
+Non-tuples form. For detailed description see theory \<open>CogentCommon_common_Tuples\<close>.
+\<close>
+
+subsection \<open>32 Bit Functions\<close>
+
+definition seq32_cnt :: "32 word \<Rightarrow> 32 word \<Rightarrow> 32 word \<Rightarrow> nat" where
+  "seq32_cnt frm to step \<equiv> ((unat to)-(unat frm)+(unat step)-1) div (unat step)"
+
+definition seq32_term :: "32 word \<Rightarrow> 32 word \<Rightarrow> bool" where 
+  "seq32_term to step \<equiv> (step > 0) \<and> ((unat to) + (unat step) \<le> 2 ^ LENGTH(32))"
+
+subsubsection \<open>seq32_simple\<close>
+
 fun seq32_simple_imp :: "nat \<Rightarrow> ('acc \<Rightarrow> 'acc) \<Rightarrow> 'acc \<Rightarrow> 'acc" where
-    "seq32_simple_imp cnt f acc = 
-      (if cnt = 0 then acc 
-       else seq32_simple_imp (cnt-1) f (f acc))"
+    "seq32_simple_imp 0 f acc = acc" |
+    "seq32_simple_imp (Suc n) f acc = f (seq32_simple_imp n f acc)"
 
-axiomatization where seq32_simple_def[simp]: 
-  "\<And>(acc::'acc) (f::'acc \<Rightarrow> 'acc). step \<noteq> 0 \<Longrightarrow> seq32_simple (Seq32SimpleParam.make frm to step f acc) = seq32_simple_imp (unat ((to - frm + step) div step)) f acc"
+axiomatization where seq32_simple_def: 
+  "\<And>(acc::'acc) (f::'acc \<Rightarrow> 'acc). seq32_term to step \<Longrightarrow> 
+     seq32_simple \<lparr>Seq32SimpleParam.frm\<^sub>f=frm, to\<^sub>f=to, step\<^sub>f=step, f\<^sub>f=f, acc\<^sub>f=acc\<rparr> \<equiv> 
+       seq32_simple_imp (seq32_cnt frm to step) f acc"
 
-fun seq32_imp :: "nat \<Rightarrow> 32 word \<Rightarrow> 32 word \<Rightarrow> ('acc, 'obsv, 'rbrk) Seq32_body \<Rightarrow> 'acc \<Rightarrow> 'obsv \<Rightarrow> ('acc, 'rbrk) LRR\<^sub>T" where
-  "seq32_imp cnt idx step f acc obsv = 
-    (if cnt = 0 then RR.make acc (Iterate ())
-     else let fres = f (Seq32_bodyParam.make acc obsv idx) 
-          in case RR.p2\<^sub>f fres of Break _ \<Rightarrow> fres
-             | Iterate() \<Rightarrow> seq32_imp (cnt-1) (idx+step) step f (RR.p1\<^sub>f fres) obsv)"
+subsubsection \<open>seq32\<close>
 
-axiomatization where seq32_step0[simp]: 
-  "\<And>(acc::'acc) (obsv::'obsv) (f::('acc, 'obsv, 'rbrk) Seq32_body) .seq32 (Seq32Param.make frm to 0 f acc obsv) = RR.make acc (Iterate())"
-axiomatization where seq32_def[simp]: 
-  "\<And>(acc::'acc) (obsv::'obsv) (f::('acc, 'obsv, 'rbrk) Seq32_body) .step \<noteq> 0 \<Longrightarrow> seq32 (Seq32Param.make frm to step f acc obsv) = seq32_imp (unat ((to - frm + step) div step)) frm step f acc obsv"
+fun seq32_imp :: "nat \<Rightarrow> ('acc, 'obsv, 'rbrk) Seq32_body \<Rightarrow> 'acc \<Rightarrow> 32 word \<Rightarrow> 32 word \<Rightarrow> 'obsv \<Rightarrow> ('acc, 'rbrk) LRR\<^sub>T" where
+    "seq32_imp 0 f acc frm step obsv = makeTup2 acc (Iterate())" |
+    "seq32_imp (Suc n) f acc frm step obsv = 
+       (let x = seq32_imp n f acc frm step obsv
+        in case p2Tup2 x of
+          Break _ \<Rightarrow> x |
+          Iterate _ \<Rightarrow> f \<lparr>Seq32_bodyParam.acc\<^sub>f = p1Tup2 x, obsv\<^sub>f = obsv, idx\<^sub>f = frm + (of_nat n)*step \<rparr>)"
+
+axiomatization where seq32_def: 
+  "\<And>(acc::'acc) (obsv::'obsv) (f::('acc, 'obsv, 'rbrk) Seq32_body). seq32_term to step \<Longrightarrow> 
+     seq32 \<lparr>Seq32Param.frm\<^sub>f=frm, to\<^sub>f=to, step\<^sub>f=step, f\<^sub>f=f, acc\<^sub>f=acc, obsv\<^sub>f=obsv\<rparr> \<equiv> 
+       seq32_imp (seq32_cnt frm to step) f acc frm step obsv"
+
+subsection \<open>64 Bit Functions\<close>
+
+text \<open>Analogous to 32 bit functions.\<close>
+
+definition seq64_cnt :: "64 word \<Rightarrow> 64 word \<Rightarrow> 64 word \<Rightarrow> nat" where
+  "seq64_cnt frm to step \<equiv> ((unat to)-(unat frm)+(unat step)-1) div (unat step)"
+
+definition seq64_term :: "64 word \<Rightarrow> 64 word \<Rightarrow> bool" where 
+  "seq64_term to step \<equiv> (step > 0) \<and> ((unat to) + (unat step) \<le> 2 ^ LENGTH(64))"
+
+subsubsection \<open>seq64\<close>
+
+fun seq64_imp :: "nat \<Rightarrow> ('acc, 'obsv, 'rbrk) Seq64_body \<Rightarrow> 'acc \<Rightarrow> 64 word \<Rightarrow> 64 word \<Rightarrow> 'obsv \<Rightarrow> ('acc, 'rbrk) LRR\<^sub>T" where
+    "seq64_imp 0 f acc frm step obsv = makeTup2 acc (Iterate())" |
+    "seq64_imp (Suc n) f acc frm step obsv = 
+       (let x = seq64_imp n f acc frm step obsv
+        in case p2Tup2 x of
+          Break _ \<Rightarrow> x |
+          Iterate _ \<Rightarrow> f \<lparr>Seq32_bodyParam.acc\<^sub>f = p1Tup2 x, obsv\<^sub>f = obsv, idx\<^sub>f = frm + (of_nat n)*step \<rparr>)"
+
+axiomatization where seq64_def: 
+  "\<And>(acc::'acc) (obsv::'obsv) (f::('acc, 'obsv, 'rbrk) Seq64_body). seq64_term to step \<Longrightarrow> 
+     seq64 \<lparr>Seq32Param.frm\<^sub>f=frm, to\<^sub>f=to, step\<^sub>f=step, f\<^sub>f=f, acc\<^sub>f=acc, obsv\<^sub>f=obsv\<rparr> \<equiv> 
+       seq64_imp (seq64_cnt frm to step) f acc frm step obsv"
 
 end
