isa/Gencot_CPointer.thy
@@ -4,13 +4,13 @@ theory Gencot_CPointer
 begin
 
 axiomatization where getPtr_def[simp]: "\<forall>x . getPtr x = CPtr.cont\<^sub>f x" 
-axiomatization where setPtr_def[simp]: "\<forall>arg . setPtr arg = RR.make (CPtr.make (RR.p2\<^sub>f arg)) ()"
+axiomatization where setPtr_def[simp]: "\<forall>arg . setPtr arg = makeTup2 (CPtr.make (p2Tup2 arg)) ()"
 axiomatization where exchngPtr_def[simp]: 
-  "\<forall> arg . exchngPtr arg = RR.make (CPtr.make (RR.p2\<^sub>f arg)) (CPtr.cont\<^sub>f (RR.p1\<^sub>f arg))"
+  "\<forall> arg . exchngPtr arg = makeTup2 (CPtr.make (p2Tup2 arg)) (CPtr.cont\<^sub>f (p1Tup2 arg))"
 axiomatization where modifyPtr_def[simp]: 
   "\<forall> arg . modifyPtr arg = 
-     (let p=RR.p1\<^sub>f arg; chf = RR.p1\<^sub>f (RR.p2\<^sub>f arg); inp = RR.p2\<^sub>f (RR.p2\<^sub>f arg);
-         chres = chf (RR.make (CPtr.cont\<^sub>f p) inp) 
-     in RR.make (CPtr.make (RR.p1\<^sub>f chres)) (RR.p2\<^sub>f chres))"
+     (let p=p1Tup2 arg; chf = p1Tup2 (p2Tup2 arg); inp = p2Tup2 (p2Tup2 arg);
+         chres = chf (makeTup2 (CPtr.cont\<^sub>f p) inp) 
+     in makeTup2 (CPtr.make (p1Tup2 chres)) (p2Tup2 chres))"
 
 end
